IMP-/IMP_Minus_Nat_Bijection.thy
@@ -5,12 +5,23 @@ theory IMP_Minus_Nat_Bijection
     "../Cook_Levin/IMP-_To_SAS+/IMP-_To_IMP--/Primitives"
 begin
 
+lemma xxx: "x \<noteq> y \<Longrightarrow> (s (x := aval a s)) y = s y"
+  by auto
+
+(*lemma AssignI'': 
+  "\<exists>s'.((x ::= a, s) \<Rightarrow>\<^bsup> 2 \<^esup> s' \<and> (s' = s (x := aval a s)))"
+  by (auto simp add: Assign eval_nat_numeral)
+*)
+
 unbundle IMP_Minus_Minus_Com.no_com_syntax
+
 unbundle Com.no_com_syntax
-                                                 
+
 record triangle_state = triangle_mul_state::mul_state triangle_a::nat triangle_triangle::nat
-                                            
+
 term Nat_Bijection.triangle
+
+find_theorems Max_Constant.all_variables
 
 (*definition triangle_IMP_Minus where "triangle_IMP_Minus \<equiv>
   [''a''] ''a'' ::= (A (V ''a'')) ;;
@@ -42,15 +53,17 @@ fun triangle_imp:: "triangle_state \<Rightarrow> triangle_state" where
      ret
   )"
 
+lemmas [simp del] = triangle_imp.simps
+
 lemma triangle_imp_correct: "triangle_triangle (triangle_imp s) = Nat_Bijection.triangle (triangle_a s)"
 proof (induction s rule: triangle_imp.induct)
   case (1 s)
   then show ?case
-    by (auto simp: triangle_def triangle_state_upd_def Let_def mul_imp_correct simp del: mul_imp.simps split: if_splits)
+    by (auto simp: triangle_imp.simps triangle_def triangle_state_upd_def Let_def mul_imp_correct split: if_splits)
 qed 
 
-fun triangle_imp_time:: "triangle_state \<Rightarrow> nat \<Rightarrow> nat" where
-"triangle_imp_time s t = 
+fun triangle_imp_time:: "nat \<Rightarrow> triangle_state \<Rightarrow> nat" where
+"triangle_imp_time t s = 
   (let
      mul_a' = triangle_a s;
      t = t + 2;
@@ -62,7 +75,7 @@ fun triangle_imp_time:: "triangle_state \<Rightarrow> nat \<Rightarrow> nat" whe
      t = t + 2;
      (triangle_mul_state::mul_state) = \<lparr>mul_a = mul_a', mul_b = mul_b', mul_c = mul_c', mul_d = mul_d'\<rparr>;
      mul_ret = (mul_imp triangle_mul_state);
-     t = t + mul_imp_time triangle_mul_state 0;
+     t = t + mul_imp_time 0 triangle_mul_state;
      triangle_triangle = mul_c mul_ret div 2;
      t = t + 2;
      triangle_a = triangle_a s;
@@ -72,10 +85,11 @@ fun triangle_imp_time:: "triangle_state \<Rightarrow> nat \<Rightarrow> nat" whe
      ret
   )"
 
+lemmas [simp del] = triangle_imp_time.simps
 
-lemma triangle_imp_time_acc: "(triangle_imp_time s (Suc t)) = Suc (triangle_imp_time s t)"
-  by (induction s "t" arbitrary:  rule: triangle_imp_time.induct)
-     (auto simp add: mul_state_upd_def Let_def eval_nat_numeral split: if_splits)
+lemma triangle_imp_time_acc: "(triangle_imp_time (Suc t) s) = Suc (triangle_imp_time t s)"
+  by (induction t s rule: triangle_imp_time.induct)
+     (auto simp add: triangle_imp_time.simps mul_state_upd_def Let_def eval_nat_numeral split: if_splits)
 
 definition triangle_IMP_minus where
 "triangle_IMP_minus \<equiv>
@@ -90,713 +104,85 @@ definition triangle_IMP_minus where
    [''mul''] ''d'' ::= (A (N 0));;
    \<comment> \<open>(mul_state::mul_state) = \<lparr>mul_a = mul_a, mul_b = mul_b, mul_c = 0, mul_d = 0\<rparr>;\<close>
    \<comment> \<open>mul_ret = (mul_imp mul_state);\<close>
-   invoke_subprogram ''mul'' mul_IMP_minus ;;
+   invoke_subprogram ''mul'' mul_IMP_minus;;
    \<comment> \<open>triangle_triangle = mul_c mul_ret div 2;\<close>
   ''triangle'' ::= [''mul''] ((V ''c'') \<then>);;
   ''a'' ::= A (V ''a'')
   )"
 
 
-definition triangle_IMP_Minus_state_transformer where "triangle_IMP_Minus_state_transformer p s \<equiv>
- (mul_IMP_Minus_state_transformer (''mul'' @ p) (triangle_mul_state s)) o
- (state_transformer p [(''a'',  triangle_a s), (''triangle'',  triangle_triangle s)])"
+(*definition triangle_IMP_Minus_state_transformer where "triangle_IMP_Minus_state_transformer p s \<equiv>
+ (state_transformer p [(''a'',  triangle_a s), (''triangle'',  triangle_triangle s)]) o
+ (mul_IMP_Minus_state_transformer (''mul'' @ p) (triangle_mul_state s))"*)
 
 definition "triangle_imp_to_HOL_state p s =
-              \<lparr>triangle_mul_state = mul_imp_to_HOL_state (''mul'' @ p) s, 
+              \<lparr>triangle_mul_state = mul_imp_to_HOL_state (p @ ''mul'') s, 
                triangle_a = s (add_prefix p ''a''), triangle_triangle = (s (add_prefix p ''triangle''))\<rparr>"
 
-(*notation add_prefix ("_ _" [1000, 61] 61) *)
+lemma triangle_imp_to_HOL_state_add_prefix: 
+  "triangle_imp_to_HOL_state (add_prefix p1 p2) s = triangle_imp_to_HOL_state p2 (s o (add_prefix p1))"
+  by (auto simp only: triangle_imp_to_HOL_state_def append.assoc[symmetric] comp_def
+                      mul_imp_to_HOL_state_add_prefix)
 
-(*lemma xxx: "aval e (s (y:= v)) = aval e s"
-  sorry*)
+(*lemma rev_add_prefix_all_variables:
+  "p1 \<noteq> [] \<Longrightarrow> (add_prefix p2 v \<notin> set (all_variables (invoke_subprogram p1 (c::pcom) p2)))"
+  nitpick
+  apply(induction p1 arbitrary: c p2)
+  subgoal by auto
+  subgoal apply auto
 
-lemma triangle_IMP_Minus_correct: 
-   "(triangle_IMP_minus p, s) 
-      \<Rightarrow>\<^bsup>triangle_imp_time (triangle_imp_to_HOL_state p s) 0\<^esup> 
-      triangle_IMP_Minus_state_transformer p (triangle_imp (triangle_imp_to_HOL_state p s)) s"
-  apply(subst triangle_imp.simps)
-  apply(subst triangle_imp_time.simps)
-  apply(subst Let_def)+
-  apply(subst triangle_IMP_minus_def)
-  apply(rule Seq')
-   apply(rule Seq')
-    apply(rule Seq')
-     apply(rule Seq')
-      apply(rule Seq')
-       apply(rule Seq')
-        apply(subst add_0)
-        apply(rule AssignI')
-        apply rule
-       apply(rule AssignI')
-       apply rule
-      apply(rule AssignI')
-      apply rule
-     apply(rule AssignI')
-     apply rule
-    apply(rule mul_IMP_minus_correct')
-    apply(simp add: triangle_imp_to_HOL_state_def mul_imp_to_HOL_state_def)
-   apply(rule AssignI')
-   apply rule
-  apply(subst triangle_IMP_Minus_state_transformer_def)
-  apply(subst comp_def)
-  apply(rule AssignI')
-  apply(subst mul_IMP_Minus_state_transformer_def)+
-  apply(subst state_transformer_commutes')
-   apply(simp add: triangle_imp_to_HOL_state_def triangle_state_upd_def Let_def
-              del: mul_imp.simps)+
+
+lemma rev_add_prefix_all_variables:"(add_prefix p v \<in> set (all_variables (invoke_subprogram p1 c p2)))
+       = (rev (add_prefix p v) \<in> set (map rev (all_variables (invoke_subprogram p1 c p2))))"
+  by auto
+*)
+
+lemma cons_append: "xs \<noteq> [] \<Longrightarrow> x # xs = [x] @ xs"
+  by simp
+
+lemma triangle_IMP_Minus_correct_function: 
+  "(triangle_IMP_minus p, s) 
+      \<Rightarrow>\<^bsup>t \<^esup> s'
+    \<Longrightarrow> s' (add_prefix p ''triangle'') = triangle_triangle (triangle_imp (triangle_imp_to_HOL_state p s))"
+  apply(simp only: triangle_IMP_minus_def triangle_imp.simps)
+  apply(erule Seq_tE)+
+  \<comment> \<open>Variables that we want to preserve: variables of this program minus the variables of the
+     program we call. If automation fails, this should be manually chosen variables.\<close>
+  apply(simp only: comp_def, erule mul_IMP_minus_correct'[where vars = "{''traingle''}"])
+  apply(drule AssignD)+
+  apply(elim conjE impE)
+  apply(auto simp: triangle_state_upd_def Let_def triangle_imp_to_HOL_state_def)[1]
+  apply(auto simp: mul_imp_to_HOL_state_def)[1]
   done
 
-lemma triangle_IMP_Minus_correct': 
-  shows
-   "\<lbrakk>s_HOL = (triangle_imp_to_HOL_state p s)\<rbrakk> \<Longrightarrow>
-   (triangle_IMP_minus p, s) 
-    \<Rightarrow>\<^bsup>(triangle_imp_time s_HOL 0)\<^esup> 
-      triangle_IMP_Minus_state_transformer p (triangle_imp s_HOL) s"
-  using triangle_IMP_Minus_correct
-  by (auto simp del: mul_imp.simps)
+lemma triangle_IMP_Minus_correct_time: 
+  "(triangle_IMP_minus p, s) 
+      \<Rightarrow>\<^bsup>t\<^esup> s'
+    \<Longrightarrow> t = triangle_imp_time 0 (triangle_imp_to_HOL_state p s)"
+  apply(simp only: triangle_IMP_minus_def)
+  apply(erule Seq_tE)+
+   apply(drule AssignD)+
+   apply(elim conjE)
+   apply(subst triangle_imp_time.simps)
+  apply(subst (asm) comp_def, erule mul_IMP_minus_correct'[where vars = "(set (all_variables (triangle_IMP_minus p))) - (set (all_variables (mul_IMP_minus p)))"])
+  \<comment> \<open>Warning: in the following, I am unfolding mul_imp_to_HOL_state_def. With more experiments, it
+      should become clear if this will cascade down multiple layers\<close>
+  apply(simp add: triangle_imp_time_acc triangle_imp_to_HOL_state_def triangle_state_upd_def)[1]
+  apply (auto simp: mul_imp_to_HOL_state_def)[1]
+  done
+
+lemma triangle_IMP_Minus_correct_effects:
+  "(triangle_IMP_minus p, s) \<Rightarrow>\<^bsup>t\<^esup> s' \<Longrightarrow> (vars \<inter> set (all_variables (triangle_IMP_minus p)) = {} \<longrightarrow> (\<forall>v\<in>vars. s v = s' v))"
+  by (auto intro: com_only_vars)
+
+lemma triangle_IMP_minus_correct':
+  "\<lbrakk>(triangle_IMP_minus p, s) \<Rightarrow>\<^bsup>t\<^esup> s';
+     \<lbrakk>t = (triangle_imp_time 0 (triangle_imp_to_HOL_state p s));
+      s' (add_prefix p ''triangle'') = triangle_triangle (triangle_imp (triangle_imp_to_HOL_state p s));
+      (vars \<inter> set (all_variables (triangle_IMP_minus p)) = {} \<Longrightarrow> (\<forall>v\<in>vars. s v = s' v))\<rbrakk>
+     \<Longrightarrow> P\<rbrakk> \<Longrightarrow> P"
+  using triangle_IMP_Minus_correct_time triangle_IMP_Minus_correct_function
+        triangle_IMP_Minus_correct_effects
+  by auto
 
-
-(*definition triangle_IMP_Minus where "triangle_IMP_Minus \<equiv>
-  [''a''] ''a'' ::= (A (V ''a'')) ;;
-  [''a''] ''b'' ::= ((V ''a'') \<oplus> (N 1)) ;;
-  invoke_subprogram ''a'' mul_IMP_minus ;;
-  ''triangle'' ::= [''a''] ((V ''c'') \<then>) ;;
-  ''a'' ::= (A (N 0))"
-
-
-
-
-thm add.commute
-lemma comp_add:"(\<lambda>x::'a::ab_semigroup_add. f (x +c)) = f o ((+) c)"
-  by (auto simp add: comp_def add.commute[symmetric])
-
-lemma poly_const:"poly ((+) c)"
-proof -
-  have 1:"poly (\<lambda>x. x)"
-    by (rule poly_linear)
-  have 2:"poly (\<lambda>x. c)" by simp
-  have "((+)c) = (\<lambda>x . x + c)"  by auto
-  moreover from 1 2 have "poly (\<lambda>x. x + c) " by auto
-  ultimately show ?thesis by auto
-qed
-find_theorems poly  "(o)" 
-
-lemma poly_shift: "poly f \<Longrightarrow> poly (\<lambda>x. f(x + c))"
-  by (subst comp_add) (auto intro: poly_const)
-
-   
-  
-
-lemma "poly (f o g) \<Longrightarrow> poly ((\<lambda>x. f(x + c)) o g)"
-  oops
-definition triangle_IMP_Minus_time where "triangle_IMP_Minus_time x \<equiv>
-  mul_IMP_Minus_time (1 + x) + 8"
-lemma "poly (triangle_IMP_Minus_time o exp2)"
-  unfolding triangle_IMP_Minus_time_def 
-  oops
-abbreviation triangle_IMP_Minus_state_transformer where 
-  "triangle_IMP_Minus_state_transformer p n  \<equiv>
-    state_transformer p [(''triangle'', triangle n), (''a'', 0)] \<circ> 
-    mul_IMP_Minus_state_transformer (''a'' @ p) n (n + 1)"
-
-lemma triangle_IMP_Minus_correct[intro]: 
-   "(triangle_IMP_Minus p, s) 
-      \<Rightarrow>\<^bsup>triangle_IMP_Minus_time (s (add_prefix p ''a''))\<^esup> 
-      triangle_IMP_Minus_state_transformer p (s (add_prefix p ''a'')) s"
-  unfolding triangle_IMP_Minus_def triangle_def triangle_IMP_Minus_time_def
-  by (fastforce intro!: terminates_in_t ime_state_intro[OF Seq])
-
-definition prod_encode_IMP_Minus where "prod_encode_IMP_Minus \<equiv>
-  [''a''] ''a'' ::= ((V ''a'') \<oplus> (V ''b'')) ;;
-  invoke_subprogram ''a'' triangle_IMP_Minus ;;
-  ''prod_encode'' ::= [''a''] (A (V ''triangle'')) ;;
-  [''a''] ''triangle'' ::= (A (N 0)) ;;
-  ''prod_encode'' ::= ((V ''a'') \<oplus> (V ''prod_encode'')) ;;
-  zero_variables [''a'', ''b'']"
-
-definition prod_encode_IMP_Minus_time where "prod_encode_IMP_Minus_time x y \<equiv>
-  triangle_IMP_Minus_time (x + y) + 8 + zero_variables_time [''a'', ''b'']"
-
-abbreviation prod_encode_IMP_Minus_state_transformer where 
-  "prod_encode_IMP_Minus_state_transformer p x y \<equiv>
-    state_transformer p [(''prod_encode'', prod_encode (x, y)), (''a'', 0), (''b'', 0)] \<circ>
-    state_transformer (''a'' @ p) [(''triangle'', 0)] \<circ> 
-    triangle_IMP_Minus_state_transformer (''a'' @ p) (x + y)"
-
-lemma prod_encode_IMP_Minus_correct[intro]: 
-  "(prod_encode_IMP_Minus p, s) 
-      \<Rightarrow>\<^bsup>prod_encode_IMP_Minus_time (s (add_prefix p ''a'')) (s (add_prefix p ''b''))\<^esup> 
-      prod_encode_IMP_Minus_state_transformer p (s (add_prefix p ''a'')) (s (add_prefix p ''b'')) s"
-  unfolding prod_encode_IMP_Minus_def prod_encode_def prod_encode_IMP_Minus_time_def
-  by(fastforce intro!: terminates_in_time_state_intro[OF Seq])
-
-fun prod_decode_aux_iterations :: "nat \<Rightarrow> nat \<Rightarrow> nat"
-  where "prod_decode_aux_iterations k m =
-    (if m \<le> k then 0 else Suc (prod_decode_aux_iterations (Suc k) (m - Suc k)))"
-
-declare prod_decode_aux_iterations.simps [simp del]
-
-definition prod_decode_aux_iteration where "prod_decode_aux_iteration \<equiv>
-  ''a'' ::= ((V ''a'') \<oplus> (N 1)) ;;
-  ''b'' ::= ((V ''b'') \<ominus> (V ''a'')) ;;
-  ''c'' ::= ((V ''b'') \<ominus> (V ''a''))"
-
-abbreviation prod_decode_aux_loop_state_transformer 
-  where "prod_decode_aux_loop_state_transformer p x y \<equiv>
-    state_transformer p [(''a'', fst (prod_decode_aux x y)
-                               + snd (prod_decode_aux x y)),
-                         (''b'', fst (prod_decode_aux x y)),
-                         (''c'', 0)]"
-
-lemma prod_decode_aux_loop_correct: 
-  "s (add_prefix p ''a'') = k \<Longrightarrow> s (add_prefix p ''b'') = m \<Longrightarrow> s (add_prefix p ''c'') = m - k 
-  \<Longrightarrow> ((WHILE ''c'' \<noteq>0 DO prod_decode_aux_iteration) p, s) 
-      \<Rightarrow>\<^bsup>2 + 7 * prod_decode_aux_iterations k m\<^esup> 
-      (if m - k \<noteq> 0 then prod_decode_aux_loop_state_transformer p k m s else s)"
-proof(induction k m arbitrary: s rule: prod_decode_aux.induct)
-  case (1 k m)
-  then show ?case
-  proof(cases "m - k")
-    case 0
-    then show ?thesis
-      using 1 terminates_in_state_intro[OF Big_StepT.WhileFalse]
-      by(auto simp:  prod_decode_aux.simps numeral_eq_Suc 
-          prod_decode_aux_iterations.simps)
-  next
-    case (Suc nat)
-
-    show ?thesis
-      apply(rule terminates_in_time_state_intro[OF Big_StepT.WhileTrue[OF _ _ "1.IH"]])
-      unfolding prod_decode_aux_iteration_def
-      using \<open>s (add_prefix p ''a'') = k\<close>  \<open>s (add_prefix p ''b'') = m\<close>  
-        \<open>s (add_prefix p ''c'') = m - k\<close> \<open>m - k = Suc nat\<close>
-        prod_decode_aux_iterations.simps[where ?k = k]
-        prod_decode_aux.simps[where ?k = k]
-        prod_decode_aux.simps[where ?k = "(Suc (s (add_prefix p ''a'')))"]
-      by fastforce+
-  qed
-qed
-
-definition fst_nat_IMP_Minus where "fst_nat_IMP_Minus \<equiv>
-  ''b'' ::= (A (V ''a'')) ;; 
-  ''a'' ::= (A (N 0)) ;;
-  ''c'' ::= ((V ''b'') \<ominus> (V ''a'')) ;;
-  WHILE ''c'' \<noteq>0 DO prod_decode_aux_iteration ;;
-  ''fst_nat'' ::= (A (V ''b'')) ;;
-  ''a'' ::= (A (N 0)) ;;
-  ''b'' ::= (A (N 0))"
-
-definition fst_nat_IMP_Minus_time where "fst_nat_IMP_Minus_time x \<equiv>
-  14 + 7 * prod_decode_aux_iterations 0 x"
-
-abbreviation fst_nat_IMP_Minus_state_transformer where "fst_nat_IMP_Minus_state_transformer p x
-  \<equiv> state_transformer p [(''a'', 0),
-                          (''b'', 0),
-                          (''c'', 0),
-                          (''fst_nat'', fst_nat x)]"
-
-lemma fst_nat_IMP_Minus_correct[intro]: 
-  "(fst_nat_IMP_Minus p, s) 
-      \<Rightarrow>\<^bsup>fst_nat_IMP_Minus_time (s (add_prefix p ''a''))\<^esup> 
-    fst_nat_IMP_Minus_state_transformer p (s (add_prefix p ''a'')) s"
-  unfolding fst_nat_IMP_Minus_def fst_nat_def fst_nat_IMP_Minus_time_def
-  by (fastforce simp: prod_decode_def prod_decode_aux.simps[of 0 0] 
-      intro!: prod_decode_aux_loop_correct
-      terminates_in_time_state_intro[OF Seq'])
-
-definition hd_IMP where "hd_IMP \<equiv>
-  [''fst''] ''a'' ::=  (V ''xs'' \<ominus> N 1) ;;
-  invoke_subprogram ''fst'' fst_nat_IMP_Minus ;;
-  ''ans'' ::= [''fst''] A (V ''fst_nat'');;
-  ''xs'' ::= A (N 0)
-"
-
-
-abbreviation hd_state_transformer where 
-"hd_state_transformer p xs \<equiv> 
-state_transformer p [(''ans'',hd_nat xs) , (''xs'',0)] o
-fst_nat_IMP_Minus_state_transformer (''fst''@ p) (xs -1)
-"
-
-definition hd_time where "
-hd_time x \<equiv> fst_nat_IMP_Minus_time (x-1) + 6 "
-
-lemma hd_nat_IMP_Minus_correct[intro]: 
-  "(hd_IMP p, s) 
-      \<Rightarrow>\<^bsup>  hd_time (s (add_prefix p ''xs''))\<^esup> 
-   hd_state_transformer p (s (add_prefix p ''xs'')) s"
-  unfolding hd_IMP_def hd_time_def  hd_nat_def
-  apply (rule terminates_in_time_state_intro)
-    apply (rule Big_StepT.Seq)+
-  by fastforce+
-  
-  
-  
-fun f::"real\<Rightarrow>real" where "f x = x^3  -4x^2 + x+3"
-
-value "f (-2)"
-value "f (4)"
-value "f ((-2* f(4) + 4*f(-2))/ (f(4)-f(-2)))"
-
-definition snd_nat_IMP_Minus where "snd_nat_IMP_Minus \<equiv>
-  ''b'' ::= (A (V ''a'')) ;; 
-  ''a'' ::= (A (N 0)) ;;
-  ''c'' ::= ((V ''b'') \<ominus> (V ''a'')) ;;
-  WHILE ''c'' \<noteq>0 DO prod_decode_aux_iteration ;;
-  ''snd_nat'' ::= ((V ''a'') \<ominus> (V ''b'')) ;;
-  ''a'' ::= (A (N 0)) ;;
-  ''b'' ::= (A (N 0))"
-
-definition snd_nat_IMP_Minus_time where "snd_nat_IMP_Minus_time x \<equiv>
-  14 + 7 * prod_decode_aux_iterations 0 x"
-
-abbreviation snd_nat_IMP_Minus_state_transformer where "snd_nat_IMP_Minus_state_transformer p x
-  \<equiv> state_transformer p [(''a'', 0),
-                          (''b'', 0),
-                          (''c'', 0),
-                          (''snd_nat'', snd_nat x)]"
-
-lemma snd_nat_IMP_Minus_correct[intro]: 
-  "(snd_nat_IMP_Minus p, s) 
-      \<Rightarrow>\<^bsup>snd_nat_IMP_Minus_time (s (add_prefix p ''a''))\<^esup> 
-    snd_nat_IMP_Minus_state_transformer p (s (add_prefix p ''a'')) s"
-  unfolding snd_nat_IMP_Minus_def snd_nat_def snd_nat_IMP_Minus_time_def
-  by (fastforce simp: prod_decode_def prod_decode_aux.simps[of 0 0] 
-      intro!: prod_decode_aux_loop_correct
-      terminates_in_time_state_intro[OF Seq'])
-
-definition tl_IMP where "tl_IMP \<equiv>
-  [''snd''] ''a'' ::=  (V ''input1'' \<ominus> N 1) ;;
-  invoke_subprogram ''snd'' snd_nat_IMP_Minus ;;
-  ''ans'' ::= [''snd''] A (V ''snd_nat'');;
-  [''snd''] ''snd_nat'' ::= A (N 0);;
-  ''input1'' ::= A (N 0)
-"
-
-
-abbreviation tl_state_transformer where 
-"tl_state_transformer p xs \<equiv> 
-state_transformer p [(''ans'',tl_nat xs) , (''xs'',0)] o
-state_transformer (''snd'' @ p) [(''snd_nat'',0)] o
-snd_nat_IMP_Minus_state_transformer (''snd''@ p) (xs -1)
-"
-
-definition tl_time where "
-tl_time x \<equiv> snd_nat_IMP_Minus_time (x-1) + 8 "
-
-lemma tl_nat_IMP_Minus_correct[intro]: 
-  "(tl_IMP p, s) 
-      \<Rightarrow>\<^bsup>  tl_time (s (add_prefix p ''xs''))\<^esup> 
-   tl_state_transformer p (s (add_prefix p ''xs'')) s"
-  unfolding tl_IMP_def tl_time_def  tl_nat_def 
-  apply (rule terminates_in_time_state_intro)
-    apply (rule Big_StepT.Seq)+
-  by fastforce+
-
-definition nth_nat_iteration where "nth_nat_iteration \<equiv>
-  [''a''] ''a'' ::= ((V ''a'') \<ominus> (N 1)) ;;
-  invoke_subprogram ''a'' snd_nat_IMP_Minus ;;
-  ''a'' ::= [''a''] (A (V ''snd_nat'')) ;;
-  [''a''] ''snd_nat'' ::= (A (N 0)) ;;
-  ''nth_nat'' ::= ((V ''nth_nat'') \<ominus> (N 1))"
-
-fun nth_nat_loop_time :: "nat \<Rightarrow> nat \<Rightarrow> nat" where
-"nth_nat_loop_time 0 x = 2" |
-"nth_nat_loop_time (Suc n) x = 9 + snd_nat_IMP_Minus_time (x - 1) 
-  + nth_nat_loop_time n (tl_nat x)"
-
-fun drop_n_nat :: "nat \<Rightarrow> nat\<Rightarrow> nat" where 
-"drop_n_nat 0 x = x "|
-"drop_n_nat (Suc n) x = drop_n_nat n (tl_nat x)"
-
-lemma nth_nat_is_hd_of_drop_n_nat:
-  "nth_nat n x = fst_nat (drop_n_nat n x - Suc 0)"
-  by (induction n arbitrary: x)
-    (auto simp: hd_nat_def)
-
-abbreviation nth_nat_loop_state_transformer where "nth_nat_loop_state_transformer p k x \<equiv>
-  (if k = 0 then (\<lambda>s. s)
-   else 
-        state_transformer p [
-        (''a'', drop_n_nat k x),
-        (''nth_nat'',  0)]
-        \<circ> state_transformer (''a'' @ p) [
-          (''snd_nat'', 0)]
-        \<circ> snd_nat_IMP_Minus_state_transformer (''a'' @ p) 0)"
-
-lemma nth_nat_loop_correct:
-  "s (add_prefix p ''nth_nat'') = k
-  \<Longrightarrow> ((WHILE ''nth_nat'' \<noteq>0 DO nth_nat_iteration) p, s) 
-      \<Rightarrow>\<^bsup>nth_nat_loop_time k (s (add_prefix p ''a''))\<^esup>
-      nth_nat_loop_state_transformer p k (s (add_prefix p ''a'')) s "
-proof(induction k arbitrary: s)
-  case 0
-  then show ?case
-    by(auto simp: numeral_eq_Suc fun_eq_iff 
-        intro!: terminates_in_state_intro[OF Big_StepT.WhileFalse])
-next
-  case (Suc k)
-  show ?case
-    apply(rule terminates_in_time_state_intro[OF Big_StepT.WhileTrue[OF _ _ Suc.IH]])
-    using \<open>s (add_prefix p ''nth_nat'') = Suc k\<close>
-    unfolding nth_nat_iteration_def
-    by (fastforce simp: tl_nat_def)+
-qed
-
-
-definition nth_nat_IMP_Minus where "nth_nat_IMP_Minus \<equiv>
-  ''nth_nat'' ::= (A (V ''a'')) ;;
-  ''a'' ::= (A (V ''b'')) ;;
-  WHILE ''nth_nat'' \<noteq>0 DO nth_nat_iteration ;;
-  [''b''] ''a'' ::= ((V ''a'') \<ominus> (N 1)) ;;
-  invoke_subprogram ''b'' fst_nat_IMP_Minus ;;
-  ''nth_nat'' ::= [''b''] (A (V ''fst_nat'')) ;;
-  [''b''] ''fst_nat'' ::= (A (N 0)) ;;
-  zero_variables [''a'', ''b'']"
-
-definition nth_nat_IMP_Minus_time where "nth_nat_IMP_Minus_time n x \<equiv>
-  10 + nth_nat_loop_time n x + fst_nat_IMP_Minus_time ((drop_n_nat n x) - 1)
-  + zero_variables_time [''a'', ''b'']"
-
-abbreviation nth_nat_IMP_Minus_state_transformer where "nth_nat_IMP_Minus_state_transformer p k x
-  \<equiv> state_transformer p [(''nth_nat'', nth_nat k x), (''a'', 0), (''b'', 0)]
-     \<circ> state_transformer (''b'' @ p) [(''fst_nat'', 0)]
-     \<circ> fst_nat_IMP_Minus_state_transformer (''b'' @ p) 0
-     \<circ> nth_nat_loop_state_transformer p k x"
-
-lemma nth_nat_IMP_Minus_correct:
-  "(nth_nat_IMP_Minus p, s) 
-    \<Rightarrow>\<^bsup>nth_nat_IMP_Minus_time (s (add_prefix p ''a'')) (s (add_prefix p ''b''))\<^esup>
-    nth_nat_IMP_Minus_state_transformer p (s (add_prefix p ''a'')) (s (add_prefix p ''b'')) s"
-  unfolding nth_nat_IMP_Minus_def nth_nat_IMP_Minus_time_def tl_nat_def 
-  by (cases "s (add_prefix p ''a'') = 0") (fastforce 
-      simp: hd_nat_def nth_nat_is_hd_of_drop_n_nat
-      intro!: terminates_in_time_state_intro[OF Seq']
-      intro: nth_nat_loop_correct)+
-
-definition cons_IMP_Minus
-  where "cons_IMP_Minus \<equiv> 
-    [''a''] ''a'' ::= (A (V ''a'')) ;;
-    [''a''] ''b'' ::= (A (V ''b'')) ;;
-    invoke_subprogram ''a'' prod_encode_IMP_Minus ;;
-    ''cons'' ::= [''a''] ((V ''prod_encode'') \<oplus> (N 1)) ;;
-    [''a''] ''prod_encode'' ::= (A (N 0)) ;;
-    zero_variables [''a'', ''b'']"
-
-definition cons_IMP_Minus_time where "cons_IMP_Minus_time h t \<equiv>
-  8 + prod_encode_IMP_Minus_time h t + zero_variables_time [''a'', ''b'']"
-
-abbreviation cons_IMP_Minus_state_transformer where "cons_IMP_Minus_state_transformer p h t
-  \<equiv> state_transformer p [(''cons'', h ## t), (''a'', 0), (''b'', 0)]
-    \<circ> state_transformer (''a'' @ p) [(''prod_encode'', 0)]
-    \<circ> prod_encode_IMP_Minus_state_transformer (''a'' @ p) h t"
-
-lemma cons_IMP_Minus_correct[intro]:
-  "(cons_IMP_Minus p, s) 
-    \<Rightarrow>\<^bsup>cons_IMP_Minus_time (s (add_prefix p ''a'')) (s (add_prefix p ''b''))\<^esup>
-     cons_IMP_Minus_state_transformer p (s (add_prefix p ''a'')) (s (add_prefix p ''b'')) s"
-  unfolding cons_IMP_Minus_def cons_IMP_Minus_time_def cons_def
-  by (fastforce intro!: terminates_in_time_state_intro[OF Seq'])
-
-fun cons_list_IMP_Minus :: "vname list \<Rightarrow> pcom" where
-"cons_list_IMP_Minus [] = SKIP" |
-"cons_list_IMP_Minus (a # as) = (if as = [] 
-  then 
-    ''cons_list'' ::= [''a''] (A (V a)) ;;
-    [''a''] a ::= (A (N 0))
-  else
-    cons_list_IMP_Minus as ;;
-    [''b''] ''a'' ::= [''a''] (A (V a)) ;; 
-    [''b''] ''b'' ::= (A (V ''cons_list'')) ;;
-    invoke_subprogram ''b'' cons_IMP_Minus ;;
-    ''cons_list'' ::= [''b''] (A (V ''cons'')) ;;
-    [''b''] ''cons'' ::= (A (N 0)) ;;
-    [''a''] a ::= (A (N 0)))" (* TODO: don't zero here: will break if variable names not distinct*)
-
-fun cons_list :: "nat list \<Rightarrow> nat" where
-"cons_list [] = 0" |
-"cons_list (a # as) = 
-  (if as = [] 
-   then a
-   else a ## cons_list as)"
-
-fun cons_list_IMP_Minus_time :: "nat list \<Rightarrow> nat" where
-"cons_list_IMP_Minus_time [] = 1" | 
-"cons_list_IMP_Minus_time (a # as) = 
-  (if as = []
-   then 4
-   else cons_list_IMP_Minus_time as + 2 + 2 + cons_IMP_Minus_time a (cons_list as) + 2 + 2 + 2)"
-
-fun cons_list_IMP_Minus_state_transformer where 
-  "cons_list_IMP_Minus_state_transformer p [] vs = (\<lambda>s. s)" |
-  "cons_list_IMP_Minus_state_transformer p (a # as) (v#vs) = (if as = [] then
-    state_transformer (''a'' @ p) [(v, 0)]
-  \<circ> state_transformer p [(''cons_list'', a)]
-    else
-  (\<lambda> s0 .
-      let s1 = cons_list_IMP_Minus_state_transformer p as vs s0;
-          s2 = state_transformer (''b'' @ p) [(''a'', s1 (add_prefix (''a'' @ p) v))] s1;
-          s3 = state_transformer (''b'' @ p) [(''b'', s2 (add_prefix p ''cons_list''))] s2;
-          s4 = cons_IMP_Minus_state_transformer (''b'' @ p) (s3 (add_prefix (''b'' @ p) ''a'')) (s3 (add_prefix (''b'' @ p) ''b'')) s3;
-          s5 = state_transformer p [(''cons_list'', s4 (add_prefix (''b'' @ p) ''cons''))] s4;
-          s6 = state_transformer (''b'' @ p) [(''cons'', 0)] s5;
-          s7 = state_transformer (''a'' @ p) [(v, 0)] s6
-  in s7 )
-  )
-"
-
-lemma auxxx: "(let s1 = t1; s2 = t2 s1; s3 = t3 s2; s4 = t4 s3;
-                s5 = t5 s4; s6 = t6 s5; s7 = t7 s6 in s7) a
- =
-(let s1 = t1; s2 = t2 s1; s3 = t3 s2; s4 = t4 s3;
-                s5 = t5 s4; s6 = t6 s5; s7 = t7 s6 in s7 a)" by simp
-
-lemma cons_list_state_arv:
-  assumes arg_def: "ar = add_prefix (''a'' @ p)"
-  assumes dist: "distinct (v#vs)"
-  shows "cons_list_IMP_Minus_state_transformer p (map (\<lambda>i. s (ar i)) vs) vs s (ar v) = s (ar v)"
-  using dist
-proof(induct vs)
-  case (Cons b' bs')
-  then have "v \<noteq> b'" by simp
-  then show ?case
-    using Cons
-      auxxx[of "cons_list_IMP_Minus_state_transformer p (map (\<lambda>i. s (ar i)) bs') bs' s"
-        "\<lambda> s1. state_transformer (''b'' @ p) [(''a'', s1 (add_prefix (''a'' @ p) b'))] s1"
-        "\<lambda> s2. state_transformer (''b'' @ p) [(''b'', s2 (add_prefix p ''cons_list''))] s2"
-        "\<lambda> s3. cons_IMP_Minus_state_transformer (''b'' @ p) (s3 (add_prefix (''b'' @ p) ''a'')) (s3 (add_prefix (''b'' @ p) ''b'')) s3"
-        "\<lambda> s4. state_transformer p [(''cons_list'', s4 (add_prefix (''b'' @ p) ''cons''))] s4"
-        "state_transformer (''b'' @ p) [(''cons'', 0)]" "state_transformer (''a'' @ p) [(b', 0)]" ] 
-    by (auto simp: arg_def)
-qed simp
-
-lemma cons_list_IMP_Minus_correct[intro]:
-  assumes "distinct vs"
-  shows
-    "(cons_list_IMP_Minus vs p, s) 
-      \<Rightarrow>\<^bsup>cons_list_IMP_Minus_time (map (\<lambda>i. s (add_prefix (''a'' @ p) i)) vs)\<^esup>
-      cons_list_IMP_Minus_state_transformer p (map (\<lambda>i. s (add_prefix (''a'' @ p) i)) vs) vs s"
-  using assms
-proof(induction vs arbitrary: s)
-  case ConsV: (Cons v vs)
-  show ?case
-  proof (cases vs)
-    case Nil
-    then show ?thesis
-      by(auto intro!: terminates_in_time_state_intro[OF Seq'])
-  next
-    case ConsB: (Cons b bs)
-    define arg where "arg \<equiv> add_prefix (''a'' @ p)"
-
-    define s1 where "s1 =
-      cons_list_IMP_Minus_state_transformer p (map (\<lambda>i. s (arg i)) vs) vs s"
-    define s2 where "s2 =
-      s1(add_prefix (''b'' @ p) ''a'' := aval (aexp_add_prefix (''a'' @ p) (A (V v))) s1)"
-    define s3 where "s3 =
-      s2(add_prefix (''b'' @ p) ''b'' := aval (aexp_add_prefix p (A (V ''cons_list''))) s2)"
-
-    have d: "distinct vs" using ConsV by simp
-
-    have "cons_list_IMP_Minus_state_transformer p (map (\<lambda>i. s (arg i)) vs) vs s (arg v) = s (arg v)"
-      using cons_list_state_arv arg_def ConsV(2) by simp
-
-    then have c1: "(s3 (add_prefix (''b'' @ p) ''a'')) = (s (arg v))"
-      by (auto simp: s3_def s2_def s1_def arg_def)
-
-    have c2a: "(s3 (add_prefix (''b'' @ p) ''b''))
-       = cons_list_IMP_Minus_state_transformer p (map (\<lambda>i. s (arg i)) vs) vs
-          s (add_prefix p ''cons_list'')"
-      using s1_def s2_def s3_def by simp
-
-    have c2b: "(vs = [] \<Longrightarrow> s (add_prefix p ''cons_list'') = 0) \<Longrightarrow>
-      cons_list_IMP_Minus_state_transformer p (map (\<lambda>i. s (arg i)) vs) vs
-          s (add_prefix p ''cons_list'') =
- (cons_list (map (\<lambda>i. s (arg i)) vs))"
-      using ConsV(2)
-    proof(induct vs rule: cons_list_IMP_Minus.induct)
-      case (2 b' bs')
-      then show ?case
-      proof(cases bs')
-        case (Cons c cs)
-        then have ih: "cons_list_IMP_Minus_state_transformer p (map (\<lambda>i. s (arg i)) bs') bs' s (add_prefix p ''cons_list'') = cons_list (map (\<lambda>i. s (arg i)) bs')"
-          using 2 by simp
-        have d: "distinct (b' # bs')" using 2(3) by simp
-        show ?thesis
-          using cons_list_state_arv[of arg, OF _ d]
-            auxxx[of "cons_list_IMP_Minus_state_transformer p (map (\<lambda>i. s (arg i)) bs') bs' s"
-              "\<lambda> s1. state_transformer (''b'' @ p) [(''a'', s1 (add_prefix (''a'' @ p) b'))] s1"
-              "\<lambda> s2. state_transformer (''b'' @ p) [(''b'', s2 (add_prefix p ''cons_list''))] s2"
-              "\<lambda> s3. cons_IMP_Minus_state_transformer (''b'' @ p) (s3 (add_prefix (''b'' @ p) ''a'')) (s3 (add_prefix (''b'' @ p) ''b'')) s3"
-              "\<lambda> s4. state_transformer p [(''cons_list'', s4 (add_prefix (''b'' @ p) ''cons''))] s4"
-              "state_transformer (''b'' @ p) [(''cons'', 0)]" "state_transformer (''a'' @ p) [(b', 0)]"] 
-            Cons ih arg_def  by simp
-      qed simp
-    qed simp
-
-    have c2: "(s3 (add_prefix (''b'' @ p) ''b'')) = (cons_list (map (\<lambda>i. s (arg i)) vs))"
-      using c2a c2b ConsB by auto
-
-    show ?thesis
-      apply(subst arg_def[symmetric])+
-
-      apply(subst cons_list_IMP_Minus.simps(2))
-      apply(subst ConsB)
-      apply(subst List.list.simps(3))
-      apply(subst HOL.if_False)
-      apply(subst List.list.map(2))
-      apply(subst cons_list_IMP_Minus_time.simps(2))
-      apply(subst ConsB)
-      apply(subst ConsB)
-      apply(subst ConsB[symmetric])
-      apply(subst List.list.map(2))
-      apply(subst List.list.simps(3))
-      apply(subst HOL.if_False)
-      apply(rule Seq')+
-            apply(subst arg_def)
-            apply(rule ConsV)
-            apply(simp add: d)
-
-           apply(subst arg_def[symmetric])
-           apply(subst s1_def[symmetric])
-
-           apply(rule terminates_in_time_state_intro[OF Big_StepT.Assign])
-            apply simp  apply(rule refl)
-          apply(subst s2_def[symmetric])
-          apply(rule terminates_in_time_state_intro[OF Big_StepT.Assign])
-           apply simp apply (rule refl)
-         apply(subst s3_def[symmetric])
-         apply(rule terminates_in_time_state_intro[OF cons_IMP_Minus_correct])
-          apply(subst c1) apply(subst c2)
-
-          apply(fastforce intro!: terminates_in_time_state_intro[OF Big_StepT.Assign]
-          simp add: ConsB Let_def
-          s3_def s2_def s1_def)+
-      done
-  qed
-qed simp
-
-
-
-definition reverse_nat_acc_IMP_Minus_iteration where "reverse_nat_acc_IMP_Minus_iteration \<equiv>
-  ''a'' ::= ((V ''f'') \<ominus> (N 1)) ;;
-  IMP_Minus_fst_nat ;;
-  
-  cons_IMP_Minus (V ''fst_nat'') (V ''e'') ;;
-
-  ''a'' ::= ((V ''f'') \<ominus> (N 1)) ;;
-  IMP_Minus_snd_nat ;;
-  
-  ''e'' ::= (A (V ''cons'')) ;;
-  ''f'' ::= (A (V ''snd_nat'')) ;;
-
-  zero_variables [''a'', ''b'', ''c'', ''d'', ''fst_nat'', ''snd_nat'', ''cons'']"
-
-definition reverse_nat_acc_IMP_Minus_iteration_time where 
-  "reverse_nat_acc_IMP_Minus_iteration_time acc n \<equiv>
-    8 + IMP_Minus_fst_nat_time (n - 1) + cons_IMP_Minus_time (hd_nat n) acc
-    + IMP_Minus_fst_nat_time (n - 1)
-    + zero_variables_time [''a'', ''b'', ''c'', ''d'', ''fst_nat'', ''snd_nat'', ''cons'']"
-
-(*"reverse_nat_acc acc e  n f =
-  (if n = 0 then acc 
-   else reverse_nat_acc ((hd_nat n) ## acc) (tl_nat n) )"*)
-
-lemma reverse_nat_acc_IMP_Minus_iteration_correct: 
-  "(reverse_nat_acc_IMP_Minus_iteration, s) 
-    \<Rightarrow>\<^bsup>reverse_nat_acc_IMP_Minus_iteration_time (s ''e'') (s ''f'')\<^esup>
-    s(''a'' := 0,
-      ''b'' := 0,
-      ''c'' := 0,
-      ''d'' := 0,
-      ''e'' := ((hd_nat (s ''f'')) ## (s ''e'')),
-      ''f'' := (tl_nat (s ''f'')),
-      ''triangle'' := 0,
-      ''prod_encode'' := 0,
-      ''cons'' := 0,
-      ''fst_nat'' := 0,
-      ''snd_nat'' := 0)"
-  unfolding reverse_nat_acc_IMP_Minus_iteration_def 
-    reverse_nat_acc_IMP_Minus_iteration_time_def
-  by(fastforce 
-       simp: hd_nat_def tl_nat_def 
-       intro!: terminates_in_time_state_intro[OF Seq']
-       intro: IMP_Minus_fst_nat_correct IMP_Minus_snd_nat_correct zero_variables_correct
-       cons_IMP_Minus_correct)
-
-(* WHILE ''f'' \<noteq>0 DO reverse_nat_acc_IMP_Minus_loop_iteration *)
-
-fun reverse_nat_acc_IMP_Minus_loop_time where 
-"reverse_nat_acc_IMP_Minus_loop_time acc n = 
-  (if n = 0 then 2 
-   else 1 + reverse_nat_acc_IMP_Minus_iteration_time acc n + 
-    reverse_nat_acc_IMP_Minus_loop_time ((hd_nat n) ## acc) (tl_nat n))"
-
-lemma reverse_nat_acc_IMP_Minus_loop_correct[intro]: 
-  "(WHILE ''f'' \<noteq>0 DO reverse_nat_acc_IMP_Minus_iteration, s) 
-    \<Rightarrow>\<^bsup>reverse_nat_acc_IMP_Minus_loop_time (s ''e'') (s ''f'')\<^esup>
-    (if s ''f'' \<noteq> 0 then
-      s(''a'' := 0,
-        ''b'' := 0,
-        ''c'' := 0,
-        ''d'' := 0,
-        ''e'' := reverse_nat_acc (s ''e'') (s ''f''),
-        ''f'' := 0,
-        ''triangle'' := 0,
-        ''prod_encode'' := 0,
-        ''cons'' := 0,
-        ''fst_nat'' := 0,
-        ''snd_nat'' := 0)
-      else s)"
-proof(induction "s ''e''" "s ''f''" arbitrary: s rule: reverse_nat_acc.induct)
-  case 1
-  then show ?case
-  proof(cases "s ''f''")
-    case 0
-    then show ?thesis
-      by (fastforce intro: terminates_in_time_state_intro[OF Big_StepT.WhileFalse])
-  next
-    case (Suc nat)
-        
-    then show ?thesis
-      by(fastforce intro!: terminates_in_time_state_intro[OF
-        Big_StepT.WhileTrue[OF _ reverse_nat_acc_IMP_Minus_iteration_correct 1(1)]])
-  qed
-qed
-
-definition "reverse_nat_acc_IMP_Minus" where "reverse_nat_acc_IMP_Minus \<equiv>
-  ''e'' ::= (A (V ''a'')) ;;
-  ''f'' ::= (A (V ''b'')) ;;
-  WHILE ''f'' \<noteq>0 DO reverse_nat_acc_IMP_Minus_iteration ;;
-  ''reverse_nat_acc'' ::= (A (V ''e'')) ;;
-  zero_variables [''a'', ''b'', ''c'', ''d'', ''fst_nat'', ''snd_nat'', ''cons'', ''e'',
-    ''triangle'', ''prod_encode'']"
-
-definition reverse_nat_acc_IMP_Minus_time where "reverse_nat_acc_IMP_Minus_time acc n \<equiv>
-  6 + reverse_nat_acc_IMP_Minus_loop_time acc n
-  + zero_variables_time 
-    [''a'', ''b'', ''c'', ''d'', ''fst_nat'', ''snd_nat'', ''cons'', ''e'',
-      ''triangle'', ''prod_encode'']"
-
-lemma reverse_nat_acc_IMP_Minus_correct:
-  "(reverse_nat_acc_IMP_Minus, s) 
-    \<Rightarrow>\<^bsup>reverse_nat_acc_IMP_Minus_time (s ''a'') (s ''b'')\<^esup>
-      s(''a'' := 0,
-        ''b'' := 0,
-        ''c'' := 0,
-        ''d'' := 0,
-        ''e'' := 0,
-        ''f'' := 0,
-        ''triangle'' := 0,
-        ''prod_encode'' := 0,
-        ''cons'' := 0,
-        ''fst_nat'' := 0,
-        ''snd_nat'' := 0,
-        ''reverse_nat_acc'' := reverse_nat_acc (s ''a'') (s ''b''))"
-  unfolding reverse_nat_acc_IMP_Minus_def reverse_nat_acc_IMP_Minus_time_def
-  apply(cases "s ''b''") 
-  by(fastforce 
-      intro!: HOL.ext terminates_in_time_state_intro[OF Seq'] 
-      zero_variables_correct reverse_nat_acc_IMP_Minus_loop_correct
-      intro:  reverse_nat_acc_IMP_Minus_loop_correct)+
-  *)
 end
