IMP-/Multiplication.thy
@@ -1,14 +1,14 @@
-\<^marker>\<open>creator Florian Kessler\<close>
+\<^marker>\<open>creator Florian Kessler, Mohammad Abdulaziz\<close>
 
 theory Multiplication
   imports Big_Step_Small_Step_Equivalence "HOL-Library.Discrete"
     Canonical_State_Transformers "../Lib/Polynomial_Growth_Functions"
 begin
 
+
 unbundle no_com_syntax
 
-(*
-definition max_a_min_b_IMP_Minus where "max_a_min_b_IMP_Minus =
+(*definition max_a_min_b_IMP_Minus where "max_a_min_b_IMP_Minus =
   ''c'' ::= ((V ''a'') \<ominus> (V ''b'')) ;;
   IF ''c''\<noteq>0 
   THEN
@@ -85,17 +85,19 @@ function mul_imp:: "mul_state \<Rightarrow> mul_state" where
 termination
   by  (relation "measure (\<lambda>s. mul_b s)") (auto simp: mul_state_upd_def Let_def split: if_splits)
 
+lemmas [simp del] = mul_imp.simps
+
 lemma mul_imp_correct: "mul_c (mul_imp s) = mul_c s + mul_a s * mul_b s"
 proof (induction s rule: mul_imp.induct)
   case (1 s)
   then show ?case
     apply(subst mul_imp.simps)
-    apply (auto simp: mul_state_upd_def Let_def simp del: mul_imp.simps split: if_splits)
+    apply (auto simp: mul_state_upd_def Let_def split: if_splits)
     by (metis (no_types, lifting) One_nat_def add.commute add_mult_distrib2 distrib_right mult.right_neutral mult_2 mult_div_mod_eq)
 qed 
 
-function mul_imp_time:: "mul_state \<Rightarrow> nat \<Rightarrow> nat" where
-"mul_imp_time s t = 
+function mul_imp_time:: "nat \<Rightarrow> mul_state\<Rightarrow> nat" where
+"mul_imp_time t s = 
 (
     (if mul_b s \<noteq> 0 then \<comment> \<open>While b \<noteq> 0\<close>
       (
@@ -109,7 +111,7 @@ function mul_imp_time:: "mul_state \<Rightarrow> nat \<Rightarrow> nat" where
           t = t + 2;
           mul_b = mul_b s div 2;
           t = t + 2;
-          next_iteration = mul_imp_time (mul_state_upd s) t
+          next_iteration = mul_imp_time t (mul_state_upd s)
         in
           next_iteration
       )
@@ -126,11 +128,13 @@ function mul_imp_time:: "mul_state \<Rightarrow> nat \<Rightarrow> nat" where
 )"
   by pat_completeness auto
 termination
-  by  (relation "measure (\<lambda>(s, t). mul_b s)") (auto simp: mul_state_upd_def Let_def split: if_splits)
+  by  (relation "measure (\<lambda>(t, s). mul_b s)") (auto simp: mul_state_upd_def Let_def split: if_splits)
 
-lemma mul_imp_time_acc: "(mul_imp_time s (Suc t)) = Suc (mul_imp_time s t)"
-  by (induction s "t" arbitrary:  rule: mul_imp_time.induct)
-     (auto simp add: mul_state_upd_def Let_def eval_nat_numeral split: if_splits)
+lemmas [simp del] = mul_imp_time.simps
+
+lemma mul_imp_time_acc: "(mul_imp_time (Suc t) s) = Suc (mul_imp_time t s)"
+  by (induction t s arbitrary:  rule: mul_imp_time.induct)
+     (auto simp add: mul_imp_time.simps mul_state_upd_def Let_def eval_nat_numeral split: if_splits)
 
 definition mul_IMP_minus where
 "mul_IMP_minus \<equiv>
@@ -146,231 +150,69 @@ definition mul_IMP_minus where
         ''b'' ::= ((V ''b'') \<then>))
   )"
 
-definition mul_IMP_Minus_state_transformer where "mul_IMP_Minus_state_transformer p s \<equiv>
+(*definition mul_IMP_Minus_state_transformer where "mul_IMP_Minus_state_transformer p s \<equiv>
   state_transformer p  
-    [(''a'', mul_a s),(''b'',  mul_b s),(''c'',  mul_c s),(''d'', mul_d s)]"
+    [(''a'', mul_a s),(''b'',  mul_b s),(''c'',  mul_c s),(''d'', mul_d s)]"*)
 
 definition "mul_imp_to_HOL_state p s =
   \<lparr>mul_a = s (add_prefix p ''a''), mul_b = (s (add_prefix p ''b'')),
    mul_c = (s (add_prefix p ''c'')), mul_d =  (s (add_prefix p ''d''))\<rparr>"
 
-lemma mul_IMP_minus_correct: 
-  shows
-   "(mul_IMP_minus p, s) 
-    \<Rightarrow>\<^bsup>(mul_imp_time (mul_imp_to_HOL_state p s) 0)\<^esup> 
-      mul_IMP_Minus_state_transformer p (mul_imp (mul_imp_to_HOL_state p s)) s"
-proof(induction "mul_imp_to_HOL_state p s" arbitrary: s rule: mul_imp.induct)
-  case 1
-  then show ?case
-    apply(subst mul_IMP_Minus_state_transformer_def)
-    apply(subst mul_imp.simps)
-    apply(subst mul_imp_time.simps)
-    apply(subst Let_def)+
-    apply(subst mul_IMP_minus_def)
-    apply(rule WhileI[where y = "mul_imp_time (mul_state_upd (mul_imp_to_HOL_state p s)) 0"])
-     apply(intro conjI)
-       apply(rule Seq')
-       apply(rule Seq')
-         apply(rule Seq')
-           apply(rule Big_StepT.Assign)
-         apply(rule IfI)
-                apply(rule Big_StepT.Assign)
-                   apply(rule Big_StepT.Assign)
-            apply rule
-            apply rule
-            apply(rule Big_StepT.Assign)
-       apply(rule Big_StepT.Assign)
-  apply(dest_com)
-  apply(simp add: mul_imp_to_HOL_state_def)
-         apply(simp add: mul_state_upd_def mul_imp_to_HOL_state_def)
-        apply(auto simp add: Let_def mul_state_upd_def mul_imp_to_HOL_state_def
-                   simp del: mul_imp.simps mul_imp_time.simps split: if_splits)[1]
-        apply(auto simp add: Let_def mul_state_upd_def mul_imp_to_HOL_state_def
-                   simp del: mul_imp.simps mul_imp_time.simps split: if_splits)[1]
-    apply (simp add: mul_state_upd_def mul_IMP_Minus_state_transformer_def)
-    apply (simp add: mul_state_upd_def mul_IMP_Minus_state_transformer_def)
-    apply (simp add: mul_state_upd_def mul_IMP_Minus_state_transformer_def)
-    apply (simp add: mul_IMP_minus_def)
-        apply(auto simp add: Let_def mul_state_upd_def mul_imp_to_HOL_state_def state_transformer_def
-                   simp del: mul_imp_time.simps split: if_splits)[1]
-        apply(auto simp add: Let_def mul_state_upd_def mul_imp_to_HOL_state_def state_transformer_def
-                   simp del: mul_imp_time.simps split: if_splits)[1]
-    apply(subst mul_imp_time_acc)+
-        apply(auto simp add: Let_def mul_state_upd_def mul_imp_to_HOL_state_def
-                   simp del: mul_imp.simps mul_imp_time.simps split: if_splits)[1]
-    apply(subst mul_imp_time_acc)+
-        apply(auto simp add: Let_def mul_state_upd_def mul_imp_to_HOL_state_def
-                   simp del: mul_imp.simps mul_imp_time.simps split: if_splits)[1]
-    done
-qed
+lemma mul_imp_to_HOL_state_add_prefix: 
+  "mul_imp_to_HOL_state (add_prefix p1 p2) s = mul_imp_to_HOL_state p2 (s o (add_prefix p1))"
+  by (auto simp: mul_imp_to_HOL_state_def)
+
+lemma mul_imp_to_HOL_state_add_prefix':
+  "mul_imp_to_HOL_state (x # p2) s = mul_imp_to_HOL_state p2 (s o (add_prefix [x]))"
+  by (auto simp: mul_imp_to_HOL_state_def)
+
+lemma mul_IMP_minus_correct_time:
+  "(mul_IMP_minus p, s) \<Rightarrow>\<^bsup>t\<^esup> s' \<Longrightarrow> t = (mul_imp_time 0 (mul_imp_to_HOL_state p s))"
+  apply(induction "mul_imp_to_HOL_state p s" arbitrary: s s' t rule: mul_imp.induct)
+  apply(simp only: mul_IMP_minus_def com_add_prefix.simps)
+  apply(erule While_tE)
+   apply(subst mul_imp_time.simps)
+   apply(auto simp: mul_imp_time_acc mul_imp_to_HOL_state_def)[1]
+  apply(dest_com')
+  apply(erule Seq_tE)+
+  apply(erule If_tE)
+   apply(drule AssignD)+
+   apply(elim conjE)
+   apply(subst mul_imp_time.simps)
+   apply(auto simp: mul_imp_time_acc mul_imp_to_HOL_state_def mul_state_upd_def)[1]
+  apply(subst mul_imp_time.simps)
+  apply(auto simp: mul_imp_time_acc mul_imp_to_HOL_state_def mul_state_upd_def)[1]
+  done
+
+lemma mul_IMP_minus_correct_function:
+  "(mul_IMP_minus p, s) \<Rightarrow>\<^bsup>t\<^esup> s' \<Longrightarrow> s' (add_prefix p ''c'') = mul_c (mul_imp (mul_imp_to_HOL_state p s))"
+  apply(induction "mul_imp_to_HOL_state p s" arbitrary: s s' t rule: mul_imp.induct)
+  apply(simp only: mul_IMP_minus_def com_add_prefix.simps)
+  apply(erule While_tE)
+   apply(subst mul_imp.simps)
+   apply(auto simp: mul_imp_to_HOL_state_def)[1]
+  apply(dest_com')
+  apply(erule Seq_tE)+
+  apply(erule If_tE)
+   apply(drule AssignD)+
+   apply(elim conjE)
+   apply(subst mul_imp.simps mul_imp_time.simps)
+   apply(auto simp: mul_imp_to_HOL_state_def mul_state_upd_def)[1]
+  apply(subst mul_imp.simps mul_imp_time.simps)
+  apply(auto simp: mul_imp_to_HOL_state_def mul_state_upd_def)[1]
+  done
+
+lemma mul_IMP_minus_correct_effects:
+  "(mul_IMP_minus p, s) \<Rightarrow>\<^bsup>t\<^esup> s' \<Longrightarrow> (vars \<inter> set (all_variables (mul_IMP_minus p)) = {} \<longrightarrow> (\<forall>v\<in>vars. s v = s' v))"
+ by (auto intro: com_only_vars)
 
 lemma mul_IMP_minus_correct':
-  shows
-   "\<lbrakk>s_HOL = (mul_imp_to_HOL_state p s)\<rbrakk> \<Longrightarrow>
-   (mul_IMP_minus p, s) 
-    \<Rightarrow>\<^bsup>(mul_imp_time s_HOL 0)\<^esup> 
-      mul_IMP_Minus_state_transformer p (mul_imp s_HOL) s"
-  using mul_IMP_minus_correct
-  by (auto simp del: mul_imp.simps)
-
-definition mul_iteration where
-"mul_iteration = 
-  ''d'' ::= ((V ''b'') \<doteq>1) ;;
-  IF ''d'' \<noteq>0
-  THEN 
-    ''c'' ::= ((V ''c'') \<oplus> (V ''a''))
-  ELSE
-    (SKIP ;; SKIP) ;;
-  ''a'' ::= ((V ''a'') \<oplus> (V ''a'')) ;;
-  ''b'' ::= ((V ''b'') \<then>) ;;
-  ''d'' ::= A (N 0)"
-
-lemma mul_iteration_effect:
-  "(mul_iteration p, s) \<Rightarrow>\<^bsup>11\<^esup> state_transformer' p
-                                 (\<lambda>s. 
-                                  [(''a'', 2 * s ''a''),
-                                   (''b'', s ''b'' div 2),
-                                   (''c'', 
-                                     (if s ''b'' mod 2 \<noteq> 0 
-                                      then s ''c'' + s ''a''
-                                      else s ''c'')),
-                                   (''d'', 0)]) s"
-    unfolding mul_iteration_def
-    by (cases "s (add_prefix p ''b'') mod 2 \<noteq> 0")
-       (fastforce intro!: terminates_in_time_state_intro[OF Seq'])+
-
-lemma mul_loop_correct:
-  assumes "s (add_prefix p ''b'') = k"
-  shows "((WHILE ''b'' \<noteq>0 DO mul_iteration) p, s) 
-    \<Rightarrow>\<^bsup>12 * (if s (add_prefix p ''b'') = 0 then 0 
-             else 1 + Discrete.log (s (add_prefix p ''b''))) + 2\<^esup> 
-    state_transformer' p
-    (\<lambda>s. [(''a'', (s ''a'') * (2 :: nat)^(if s ''b'' = 0 then 0 else 1 + Discrete.log (s ''b''))),
-          (''b'', 0),
-          (''c'', s ''c'' + s ''a'' * s ''b''),
-          (''d'', (if s ''b'' = 0 then s ''d'' else 0))]) s"
-  using assms
-proof(induction k arbitrary: s rule: less_induct )
-  case (less x)
-  thus ?case
-  proof (cases x)
-  next
-    case (Suc nat)
-
-    show ?thesis
-      apply(rule terminates_in_time_state_intro[OF Big_StepT.WhileTrue[
-              OF _ mul_iteration_effect less.IH[where ?y = "x div 2"]]])
-      using \<open>x = Suc nat\<close> \<open>s (add_prefix p ''b'') = x\<close> log_rec 
-           apply auto
-        apply(auto 
-          simp add: Euclidean_Division.div_eq_0_iff 
-          intro!: HOL.ext)
-       apply(presburger)
-      using odd_two_times_div_two_nat[where ?n=nat] mult.commute
-      by (smt (z3) One_nat_def Suc_pred mult.assoc mult_Suc_right)
-  qed (force intro: terminates_in_state_intro)
-qed
-
-definition mul_IMP_minus where "mul_IMP_minus =
-  ''c'' ::= A (N 0) ;;
-  WHILE ''b'' \<noteq>0 DO mul_iteration ;;
-  ''a'' ::= A (N 0) ;;
-  ''d'' ::= A (N 0)" 
-
-definition mul_IMP_Minus_time :: "nat \<Rightarrow> nat" where "mul_IMP_Minus_time y 
-  \<equiv> 12 * (if y = 0 then 0 else 1 + Discrete.log y) + 8"
-
-definition exp2::"nat\<Rightarrow>nat"  where "exp2 y \<equiv> 2^y"
-
-lemma log_exp_id: "Discrete.log  (exp2 x) = id x"
-  apply(induct x)
-  unfolding exp2_def by auto
-
-
-lemma exp2_0: "exp2 x \<noteq> 0"
-  unfolding exp2_def
+  "\<lbrakk>(mul_IMP_minus p, s) \<Rightarrow>\<^bsup>t\<^esup> s';
+     \<lbrakk>t = (mul_imp_time 0 (mul_imp_to_HOL_state p s));
+      s' (add_prefix p ''c'') = mul_c (mul_imp (mul_imp_to_HOL_state p s));
+      (vars \<inter> set (all_variables (mul_IMP_minus p)) = {} \<Longrightarrow> (\<forall>v\<in>vars. s v = s' v))\<rbrakk>
+     \<Longrightarrow> P\<rbrakk> \<Longrightarrow> P"
+  using mul_IMP_minus_correct_time mul_IMP_minus_correct_function mul_IMP_minus_correct_effects
   by auto
 
-lemma poly_general_form:"poly (\<lambda>x. a*x+b)"
-proof
-  show "poly ((*) a)"
-  proof (induct a)
-    case 0
-    then show ?case by auto
-  next
-    case (Suc a)
-    have distrib_add: "((*) (Suc a)) = (\<lambda>x. (*) a x + x)" by auto
-    from Suc have "poly (\<lambda>x. (*) a x)" by simp
-    moreover have "poly (\<lambda>x. x)"  by (simp add: poly_linear)
-    ultimately have "poly  (\<lambda>x. (*) a x + x)" by (simp add: poly_add)
-    with distrib_add show ?case by simp 
-  qed
-next
-  show "poly (\<lambda>x. b)" by simp
-qed
-
-lemma poly_intro: "(\<forall>x. f x = a*x + b) \<Longrightarrow> poly f"
-proof -
-  assume "\<forall>x. f x = a*x + b"
-  hence "f = (\<lambda>x . a*x+b)" by auto
-  with poly_general_form show "poly f" by auto
-qed
-
-lemma "poly (mul_IMP_Minus_time o exp2)"
-  unfolding mul_IMP_Minus_time_def comp_def log_exp_id
-  apply (auto simp add: exp2_0 )
-  apply (rule poly_intro)
-  by (auto simp add:algebra_simps)
-
-definition polye:: "(nat \<Rightarrow>nat) \<Rightarrow> bool" where 
-"polye f \<equiv> poly (f o exp2)"
-
-lemma polye_comp1: 
-"poly g \<Longrightarrow> polye f \<Longrightarrow> polye (g o f)"
-  unfolding polye_def 
-  by (simp add: comp_assoc poly_compose)
-
-lemma polye_comp2: 
-"mono f \<Longrightarrow> polye f \<Longrightarrow> polye (\<lambda>x . f (x + b))"
-  unfolding polye_def  exp2_def comp_def
-  oops
-
-abbreviation mul_IMP_Minus_state_transformer where "mul_IMP_Minus_state_transformer p a b \<equiv>
-  state_transformer p  
-    [(''a'', 0),
-     (''b'', 0),
-     (''c'',  a * b),
-     (''d'', 0)]" 
-
-lemma IMP_minus_mul_correct[intro]: 
-  shows "(mul_IMP_minus p, s) 
-    \<Rightarrow>\<^bsup>mul_IMP_Minus_time (s (add_prefix p ''b''))\<^esup> 
-      mul_IMP_Minus_state_transformer p (s (add_prefix p ''a'')) (s (add_prefix p ''b'')) s"
-  unfolding mul_IMP_Minus_time_def mul_IMP_minus_def
-  by(fastforce
-      intro!: terminates_in_time_state_intro[OF Seq']
-      intro: mul_loop_correct)
-
-fun zero_variables where
-"zero_variables [] = SKIP" |
-"zero_variables (a # as) = (a ::= (A (N 0)) ;; zero_variables as)"
-
-definition zero_variables_time where "zero_variables_time vs \<equiv>
-  1 + 2 * length vs"
-
-lemma zero_variables_correct[intro]:
-  "(zero_variables vs p, s) 
-    \<Rightarrow>\<^bsup>zero_variables_time vs\<^esup> 
-      state_transformer p (map (\<lambda>v. (v, 0)) vs) s"
-proof (induction vs arbitrary: s)
-  case (Cons a vs)
-  show ?case
-    by(auto 
-        intro!: terminates_in_state_intro[OF Seq[OF Big_StepT.Assign Cons.IH]] 
-        simp: zero_variables_time_def map_add_def
-        split: option.splits
-        dest!: map_of_SomeD)
-qed (auto simp: zero_variables_time_def)
-
-declare zero_variables.simps [simp del]
 end
